analysisByF/breakLinAVG.dfy
@@ -1,0 +1,127 @@
+ 
+include "../theory/complexity.dfy"
+include "../theory/mathSum.dfy"
+
+ghost function T(N:nat, i:nat) : nat
+  requires 0 <= i < N
+{
+  i+1
+}
+
+ghost method breakLinAVG(N:nat, P:nat->bool)
+  returns (t:nat)
+  requires N > 0
+  requires exists i :: 0 <= i < N && P(i)
+  ensures  exists k :: 0 <= k < N && P(k) && t == T(N,k)
+{
+  var i;
+  i, t := 0, 1;
+  while i != N && !P(i) 
+    invariant 0 <= i <= N
+    invariant forall j :: 0 <= j < i ==> !P(j)
+    invariant exists k :: i <= k < N && P(k)
+    invariant t == i+1
+    decreases N - i
+  {
+    i := i + 1;
+    t := t + 1;
+  }
+  assert P(i) && t == T(N,i);
+} 
+
+ghost function Tavg(N:nat) : R0
+{
+  (N + 1) as real / 2.0
+}
+
+ghost method expectationLoop(N:nat)
+  returns (tE:real)
+  requires N > 0
+  ensures tE == Tavg(N)
+  ensures tIsBigOR0(N, tE, n => n as R0)
+{
+  tE := 0.0; 
+  var p := 0; reveal sumr();  
+  while p < N
+    invariant 0 <= p <= N
+    invariant tE == sumr(0, p-1, i => (i+1) as real * (1.0 / N as real))
+    decreases N - p
+  {
+    // Run the algorithm in scenario where P(p) holds
+    var pred := inputScenario(N, p); 
+    ghost var t := breakLinAVG(N, pred); 
+    assert exists k :: 0 <= k < N && pred(k) && t == k+1;
+    assert t == T(N,p);
+    
+    // Add weighted contribution to expectation
+    lem_sumr_dropLastAll(0, p-1);
+    tE := tE + t as real * probability(N,pred,p);
+    p  := p + 1;
+  }
+  assert tE == sumr(0, N-1, i => (i+1) as real * (1.0 / N as real)); 
+  assert tE == Tavg(N) by { lem_solveSum(N); }
+
+  assert bigOR0(Tavg, n => n as R0) by { var c, n0 := lem_TavgBigOR0lin(); }
+}
+
+ghost function probability(N:nat, pred:nat->bool, p:nat) : R0
+  requires 0 <= p < N
+  requires pred(p) && forall k :: 0 <= k < N && pred(k) ==> k == p
+{
+  1.0 / N as R0
+}
+
+ghost method inputScenario(N:nat, p:nat) returns (pred0:nat->bool)
+  requires N > 0
+  requires 0 <= p < N
+  ensures pred0(p)
+  ensures forall k :: 0 <= k < N && pred0(k) ==> k == p
+{
+  assume {:axiom} exists pred:nat->bool :: pred(p) && forall k :: 0 <= k < N && pred(k) ==> k == p;
+  pred0 :| pred0(p) && forall k :: 0 <= k < N && pred0(k) ==> k == p;
+}
+
+lemma lem_solveSum(N:nat)
+  requires N > 0
+  ensures Tavg(N) == sumr(0, N-1, i => (i+1) as real * (1.0 / N as real))
+{ 
+  var c:real := 1.0 / N as real; 
+  calc {
+       sumr(0, N-1, i => (i+1) as real * c);
+    == { assert forall k:int :: 0<=k<=N-1 ==>   
+           (i => (i+1) as real * c)(k) == (l => c*(i => (i+1) as real)(l))(k);
+         lem_sumr_leibniz(0, N-1, i => (i+1) as real * c, 
+                                  l => c*(i => (i+1) as real)(l)); }
+       sumr(0, N-1, l => c*(i => (i+1) as real)(l));
+    == { lem_sumr_linearityConst(0, N-1, c, i => (i+1) as real); }
+       c * sumr(0, N-1, i => (i+1) as real);
+    == { lem_sumr_shiftIndex(0, N-1, 1, i => (i+1) as real); }
+       c * sumr(1, N, i => (i => (i+1) as real)(i-1));
+    == { assert forall k:int :: 1<=k<=N ==> 
+           (i => ((i-1)+1) as real)(k) == (i => i as real)(k);
+         lem_sumr_leibniz(1, N, i => (i => (i+1) as real)(i-1), i => i as real); }
+       c * sumr(1, N, i => i as real);
+    == { lem_sumr_interval(1, N); }
+       c * ((N*(N+1) + 1*(1-1)) as real / 2.0);
+    == c * ((N*(N+1)) as real / 2.0);  
+    == (1.0 / N as real) * ((N*(N+1)) as real / 2.0); 
+    == (N + 1) as real / 2.0;
+  }
+} 
+
+lemma lem_TavgBigOR0lin() returns (c:R0, n0:nat)
+  ensures bigOR0from(c, n0, Tavg, n => n as R0)
+{
+  // we show that c=1 and n0=1
+  c, n0 := 1.0, 1;
+  forall n:nat | 0 <= n0 <= n
+    ensures Tavg(n) <= c*(n => n as R0)(n)
+  {
+    calc {
+         Tavg(n);
+      == (n + 1) as real / 2.0;
+      <= n as real;
+    }
+    assert Tavg(n) <= c*(n => n as R0)(n); 
+  }
+}
