caseStudy/lsAVG.dfy
@@ -1,0 +1,147 @@
+
+include "../theory/complexity.dfy"
+include "../theory/mathSum.dfy"
+
+predicate inv(s:seq<int>, x:int, i:nat, N:int)
+{
+     0 <= i <= N && N <= |s|
+  && (0 <= N < |s| ==> s[i] == x)      
+  && (N == |s|     ==> (forall j :: 0 <= j < i ==> s[j] != x))
+}
+
+predicate post(s:seq<int>, x:int, i:nat)
+{
+     (0 <= i < |s| ==> s[i] == x)
+  && (i == |s|     ==> (forall j :: 0 <= j < |s| ==> s[j] != x))
+}
+
+ghost function T(s:seq<int>, x:int, i:nat) : nat
+  requires 0 <= i < |s|
+  requires s[i] == x
+{
+  i+1
+}
+
+ghost method linearSearch(s:seq<int>, x:int)
+  returns (i:nat, t:nat)
+  requires x in s
+  ensures  post(s, x, i)
+  ensures  exists k :: 0 <= k < |s| && s[k] == x && t == T(s, x, k)
+{
+  var N;
+  i, N, t := 0, |s|, 1;
+  while i != N && s[i] != x
+    invariant inv(s, x, i, N)
+    invariant forall j :: 0 <= j < i ==> s[j] != x
+    invariant exists k :: i <= k < |s| && s[k] == x
+    invariant t == i+1
+    decreases N - i
+  {
+    i := i + 1;
+    t := t + 1;
+  }
+  assert s[i] == x && t == T(s,x,i);
+} 
+ 
+
+ghost function Tavg(N:nat) : R0
+{
+  (N + 1) as real / 2.0
+}
+
+ghost method expectationLoop(N:nat)
+  returns (tE:real)
+  requires N > 0
+  ensures tE == Tavg(N)
+  ensures tIsBigOR0(N, tE, n => n as R0)
+{
+  tE := 0.0; 
+  var p := 0; reveal sumr();  
+  while p < N
+    invariant 0 <= p <= N
+    invariant tE == sumr(0, p-1, i => (i+1) as real * (1.0 / N as real))
+    decreases N - p
+  {
+    // Run algorithm in scenario where s[p] == x
+    var s, x := inputScenario(N, p); 
+    var _, t := linearSearch(s, x); 
+    assert exists k :: 0 <= k < |s| && s[k] == x && t == k+1;
+    assert t == T(s,x,p);
+    
+    // Add weighted contribution to expectation
+    lem_sumr_dropLastAll(0, p-1);
+    tE := tE + t as real * probability(s,x,p);
+    p  := p + 1;
+  }
+  assert tE == sumr(0, N-1, i => (i+1) as real * (1.0 / N as real)); 
+  assert tE == Tavg(N) by { lem_solveSum(N); }
+
+  assert bigOR0(Tavg, n => n as R0) by { var c, n0 := lem_TavgBigOR0lin(); }
+}
+
+ghost function probability(s:seq<int>, x:int, p:nat) : R0
+  requires 0 <= p < |s|
+  requires forall i, j :: 0 <= i < j < |s| ==> s[i] != s[j]
+  requires s[p] == x
+{
+  1.0 / |s| as R0
+}
+
+ghost method inputScenario(N:nat, p:nat) returns (s0:seq<int>, x0:int)
+  requires N > 0
+  requires 0 <= p < N
+  ensures  |s0| == N
+  ensures  forall i, j :: 0 <= i < j < |s0| ==> s0[i] != s0[j]
+  ensures  s0[p] == x0
+{
+  assume {:axiom} 
+    exists s:seq<int> :: |s| == N && (forall i, j :: 0 <= i < j < N ==> s[i] != s[j]);
+  s0 :| |s0| == N && forall i, j :: 0 <= i < j < N ==> s0[i] != s0[j];
+  assume {:axiom} 
+    exists x:int :: s0[p] == x;
+  x0 :| s0[p] == x0;
+}
+
+lemma lem_solveSum(N:nat)
+  requires N > 0
+  ensures Tavg(N) == sumr(0, N-1, i => (i+1) as real * (1.0 / N as real))
+{ 
+  var c:real := 1.0 / N as real; 
+  calc {
+       sumr(0, N-1, i => (i+1) as real * c);
+    == { assert forall k:int :: 0<=k<=N-1 ==>   
+          (i => (i+1) as real * c)(k) == (l => c*(i => (i+1) as real)(l))(k);
+         lem_sumr_leibniz(0, N-1, i => (i+1) as real * c, 
+                                  l => c*(i => (i+1) as real)(l)); }
+       sumr(0, N-1, l => c*(i => (i+1) as real)(l));
+    == { lem_sumr_linearityConst(0, N-1, c, i => (i+1) as real); }
+       c * sumr(0, N-1, i => (i+1) as real);
+    == { lem_sumr_shiftIndex(0, N-1, 1, i => (i+1) as real); }
+       c * sumr(1, N, i => (i => (i+1) as real)(i-1));
+    == { assert forall k:int :: 1<=k<=N ==> (i => ((i-1)+1) as real)(k) == (i => i as real)(k);
+         lem_sumr_leibniz(1, N, i => (i => (i+1) as real)(i-1), i => i as real); }
+       c * sumr(1, N, i => i as real);
+    == { lem_sumr_interval(1, N); }
+       c * ((N*(N+1) + 1*(1-1)) as real / 2.0);
+    == c * ((N*(N+1)) as real / 2.0);  
+    == (1.0 / N as real) * ((N*(N+1)) as real / 2.0); 
+    == (N + 1) as real / 2.0;
+  }
+} 
+
+lemma lem_TavgBigOR0lin() returns (c:R0, n0:nat)
+  ensures bigOR0from(c, n0, Tavg, n => n as R0)
+{
+  // we show that c=1 and n0=1
+  c, n0 := 1.0, 1;
+  forall n:nat | 0 <= n0 <= n
+    ensures Tavg(n) <= c*(n => n as R0)(n)
+  {
+    calc {
+         Tavg(n);
+      == (n + 1) as real / 2.0;
+      <= n as real;
+    }
+    assert Tavg(n) <= c*(n => n as R0)(n); 
+  }
+}
