theory/mathSum.dfy
@@ -1,0 +1,383 @@
+include "./math.dfy"
+
+/**************************************************************************
+  Sum over integer intervals
+**************************************************************************/
+
+// sum_{k=a}^{b}f(k)
+opaque ghost function sumr(a:int, b:int, f:int->real): real
+  decreases b - a
+{
+  if a > b  
+  then 0.0
+  else f(a) + sumr(a+1, b, f)
+}
+
+// a <= b+1 ==> sum_{k=a}^{b+1}f(k) = sum_{k=a}^{b}f(k) + f(b+1)
+lemma lem_sumr_dropLast(a:int, b:int, f:int->real)
+  requires a <= b+1
+  ensures  sumr(a, b+1, f) == sumr(a, b, f) + f(b+1) 
+  decreases b - a
+{ 
+  if a == b+1 {   
+    // BC: a > b
+    calc {
+         sumr(b+1, b+1, f);
+      == { reveal sumr(); }
+         f(b+1);
+      == 0.0 + f(b+1) ;
+      == { reveal sumr(); }
+         sumr(a, b, f) + f(b+1) ;       
+    }
+  } else {  
+    // Step. a <= j
+    //   IH: sum(a+1, b+1, f) = sum(a+1, b, f) + f(b+1)
+    //    T: sum(a, b+1, f)   = sum(a, b, f)   + f(b+1)
+    calc {  
+         sumr(a, b+1, f);
+      == { reveal sumr(); } 
+         f(a) + sumr(a+1, b+1, f);
+      == { lem_sumr_dropLast(a+1, b, f); }  // by IH
+         f(a) + (sumr(a+1, b, f) + f(b+1));
+      == (f(a) + sumr(a+1, b, f)) + f(b+1);
+      == { reveal sumr(); }
+         sumr(a, b, f) + f(b+1);           
+    }
+  }
+} 
+
+lemma lem_sumr_dropLastAll(a:int, b:int)
+  requires a <= b+1
+  ensures  forall f:int->real :: sumr(a, b+1, f) == sumr(a, b, f) + f(b+1) 
+{ 
+  forall f:int->real
+    ensures sumr(a, b+1, f) == sumr(a, b, f) + f(b+1) 
+  {
+     lem_sumr_dropLast(a, b, f);
+  }
+}
+
+// i <= j+1 ==> c*sum_{k=i}^{j}f(k) = sum_{k=i}^{j}c*f(k)
+lemma lem_sumr_linearityConst(a:int, b:int, c:real, f:int->real)
+  requires a <= b+1
+  ensures  c*sumr(a, b, f) == sumr(a, b, k => c*f(k))
+  decreases b - a
+{ 
+  if a == b+1 {   
+    // BC: a > b
+    calc {
+         c*sumr(b+1, b, f);
+      == { reveal sumr(); }
+         0.0;
+      == { reveal sumr(); }
+         sumr(b+1, b, k => c*f(k));       
+    }
+  } else {  
+    // Step. a <= b
+    //   IH: c*sum(a+1, b, f) = c*sum(a+1, b, k => c*f(k))
+    //    T: c*sum(a, b, f)   = c*sum(a, b, k => f(k))
+    calc {  
+         c*sumr(a, b, f);
+      == { reveal sumr(); } 
+         c*(f(a) + sumr(a+1, b, f));
+      == c*f(a) + c*sumr(a+1, b, f);         
+      == { lem_sumr_linearityConst(a+1, b, c, f); }  // by IH
+         c*f(a) + sumr(a+1, b, k => c*f(k)); 
+      == (k => c*f(k))(a) + sumr(a+1, b, k => c*f(k));
+      == { reveal sumr(); } 
+         sumr(a, b, k => c*f(k));           
+    } 
+  }  
+}
+
+// a <= b+1 ==> sum_{k=a}^{b}c = c*(b - a + 1)
+lemma lem_sumr_const(a:int, b:int, c:real)
+  requires a <= b+1
+  ensures  sumr(a, b, k => c) == c * (b - a + 1) as real
+  decreases b - a
+{ 
+  if a == b+1 {   
+    // BC: a > b
+    calc {
+         sumr(b+1, b, k => c); 
+      == { reveal sumr(); } 
+         0.0; 
+      == (b - (b+1) + 1) as real;
+    }
+  } else {  
+    // Step. a <= b
+    //   IH: sum(a+1, b, k => c) = c*(b - (a+1) + 1) = c*(b - a)
+    //    T: sum(a, b, k => c)   = c*(b - a + 1) 
+    calc {  
+         sumr(a, b, k => c);
+      == { reveal sumr(); }
+         c + sumr(a+1, b, x => c);
+      == { lem_sumr_const(a+1, b, c); }  // by IH
+         (c + c* (b - (a+1) + 1) as real);
+      == c + c*((b - a) as real);      
+      == c* (b - a + 1) as real;             
+    }
+  }
+}
+
+lemma lem_sumr_constAll(a:int, b:int)
+  requires a <= b+1
+  ensures  forall c:real :: sumr(a, b, k => c) == c * (b - a + 1) as real
+{ 
+  forall c:real
+    ensures sumr(a, b, k => c) == c * (b - a + 1) as real
+  {
+     lem_sumr_const(a, b, c);
+  }
+} 
+
+// a <= b+1 ==> sum_{k=a}^{b}f(k) = sum_{k=a+d}^{b+d}f(k-d)
+lemma lem_sumr_shiftIndex(a:int, b:int, d:int, f:int->real)
+  requires a <= b+1
+  ensures  sumr(a, b, f) == sumr(a+d, b+d, k => f(k-d))
+  decreases b - a
+{ 
+  if a == b+1 {   
+    // BC: a > b
+    calc {
+         sumr(b+1, b, f);
+      == { reveal sumr(); }
+         0.0;
+      == { reveal sumr(); }
+         sumr(b+1+d, b+d, k => f(k-d));       
+    }
+  } else {  
+    // Step. a <= b
+    //   IH: sum(a+1, b, f) = sum((a+d)+1, b+d, k => f(k-d))
+    //    T: sum(a, b, f)   = sum(a+d, b+d, k => f(k-d))
+    calc {  
+         sumr(a, b, f);
+      == { reveal sumr(); } 
+         f(a) + sumr(a+1, b, f);
+      == { lem_sumr_shiftIndex(a+1, b, d, f); }  // by IH
+         f(a) + sumr(a+1+d, b+d, k => f(k-d));
+      == (k => f(k-d))(a+d) + sumr((a+d)+1, b+d, k => f(k-d));
+      == { reveal sumr(); }
+         sumr(a+d, b+d, k => f(k-d));           
+    }
+  }
+} 
+
+// a <= b+1 ==> sum_{k=a}^{b}k = (b*(b+1) + a*(1-a))/2 
+lemma lem_sumr_interval(a:int, b:int)
+  requires a <= b+1 
+  decreases b - a
+  ensures sumr(a, b, k => k as real) == (b*(b+1) + a*(1-a)) as real / 2.0
+{ 
+  if a == b+1 {   
+    // BC: a > b
+    calc {
+         sumr(b+1, b, k => k as real);
+      == { reveal sumr(); }
+         0.0;
+      == (b*(b+1) + ((b+1))*(1-((b+1)))) as real / 2.0;
+    }
+  } else {  
+    // Step. a <= b
+    //   IH: sumr(a+1, b, K => k) = (b*(b+1) + (a+1)*(1-(a+1)))/2 
+    //    T: sumr(a, b, k => k)   = (b*(b+1) + a*(1-a))/2 
+    calc {  
+         sumr(a, b, k => k as real);
+      == { reveal sumr(); }
+         a as real + sumr(a+1, b, k => k as real);
+      == { lem_sumr_interval(a+1, b); }  // by IH
+         a as real + (b*(b+1) + (a+1)*(1-(a+1))) as real / 2.0;
+      == (b*(b+1) + a*(1-a)) as real / 2.0;            
+    }
+  } 
+}
+
+// a <= b+1 /\ (∀ k : a<=k<=b : f(k) == g(k)) 
+//          ==> sum_{k=a}^{b}f = sum_{k=a}^{b}g
+lemma lem_sumr_leibniz(a:int, b:int, f:int->real, g:int->real)
+  requires a <= b+1
+  requires forall k:int :: a<=k<=b ==> f(k) == g(k)
+  ensures sumr(a, b, f) == sumr(a, b, g)
+  decreases b - a
+{
+  if a == b+1 {   
+    // BC: a > b
+    calc {
+         sumr(b+1, b, f);
+      == { reveal sumr(); }
+         0.0;
+      == { reveal sumr(); }
+         sumr(b+1, b, g);       
+    }
+  } else {  
+    // Step. a <= b
+    //   IH: sumr(a+1, b, f) = sumr(a+1, b, g)
+    //    T: sumr(a, b, f)   = sumr(a, b, g)
+    calc {  
+         sumr(a, b, f);
+      == { reveal sumr(); } 
+         f(a) + sumr(a+1, b, f);
+      == g(a) + sumr(a+1, b, f);
+      == { lem_sumr_leibniz(a+1, b, f, g); }  // by IH
+         g(a) + sumr(a+1, b, g);
+      == { reveal sumr(); }
+         sumr(a, b, g);           
+    }
+  }
+} 
+
+/**************************************************************************
+  A special version of Sum on integer codomain
+**************************************************************************/
+ 
+// sum_{k=a}^{b}f(k)
+opaque ghost function sum(a:int, b:int, f:int->int) : int
+  decreases b - a
+{
+  if a > b  
+  then 0
+  else f(a) + sum(a+1, b, f)
+}
+
+lemma lem_sum_liftEq(a:int, b:int, f:int->int)
+  requires a <= b+1
+  ensures  sumr(a, b, liftCi2r(f)) == sum(a, b, f) as real
+  decreases b - a
+{
+  reveal sum(), sumr();
+}  
+
+// a <= b+1 ==> sum_{k=a}^{b+1}f(k) = sum_{k=a}^{b}f(k) + f(b+1)
+lemma lem_sum_dropLast(a:int, b:int, f:int->int)
+  requires a <= b+1
+  ensures  sum(a, b+1, f) == sum(a, b, f) + f(b+1) 
+{ 
+  var fr := liftCi2r(f);
+  lem_sumr_dropLast(a, b, fr);
+  assert sumr(a, b+1, fr) == sumr(a, b, fr) + fr(b+1);
+  lem_sum_liftEq(a, b+1, f);
+  lem_sum_liftEq(a, b, f);
+}
+
+lemma lem_sum_dropLastAll(a:int, b:int)
+  requires a <= b+1
+  ensures  forall f:int->int :: sum(a, b+1, f) == sum(a, b, f) + f(b+1) 
+{ 
+  forall f:int->int
+    ensures sum(a, b+1, f) == sum(a, b, f) + f(b+1) 
+  {
+     lem_sum_dropLast(a, b, f);
+  }
+}
+
+// a <= b+1 ==> sum_{k=a}^{b}c = c*(b - a + 1)
+lemma lem_sum_const(a:int, b:int, c:int)
+  requires a <= b+1
+  ensures  sum(a, b, k => c) == c*(b - a + 1)
+{ 
+  var fr := liftCi2r(k => c);
+  var c' := c as real;
+  assert c' == c as real;
+  lem_sumr_const(a, b, c');
+  assert sumr(a, b, k => c') == (c*(b - a + 1)) as real;
+  lem_sum_liftEq(a, b, k => c);
+  assert sumr(a, b, fr) == sum(a, b, k => c) as real;
+  assert sumr(a, b, fr) == sumr(a, b, k => c')
+   by { assert forall k:int :: a<=k<=b ==> c as real == c';
+        lem_sumr_leibniz(a, b, fr, k => c'); } 
+} 
+
+lemma lem_sum_constAll(a:int, b:int)
+  requires a <= b+1
+  ensures forall c:int :: sum(a, b, k => c) == (c*(b - a + 1))
+{ 
+  forall c:int
+    ensures sum(a, b, k => c) == (c*(b - a + 1))
+  {
+     lem_sum_const(a, b, c);
+  }
+} 
+
+// a <= b+1 /\ (∀ k : a<=k<=b : f(k) == g(k)) 
+//          ==> sum_{k=a}^{b}f = sum_{k=a}^{b}g
+lemma lem_sum_leibniz(a:int, b:int, f:int->int, g:int->int)
+  requires a <= b+1
+  requires forall k:int :: a<=k<=b ==> f(k) == g(k)
+  ensures  sum(a, b, f) == sum(a, b, g)
+{
+  var fr := liftCi2r(f);
+  var gr := liftCi2r(g);
+  lem_sumr_leibniz(a, b, fr, gr);
+  assert sumr(a, b, fr) == sumr(a, b, gr);
+  lem_sum_liftEq(a, b, f);
+  lem_sum_liftEq(a, b, g);
+}
+
+// a <= b+1 ==> sum_{k=a}^{b}k = (b*(b+1) + a*(1-a))/2 
+lemma lem_sum_interval(a:int, b:int)
+  requires a <= b+1 
+  decreases b - a
+  ensures sum(a, b, k => k) == (b*(b+1) + a*(1-a))/2
+{ 
+  if a == b+1 {   
+    // BC: a > b
+    calc {
+         sum(b+1, b, k => k);
+      == { reveal sum(); }
+         0;
+      == (b*(b+1) + ((b+1))*(1-((b+1))))/2;
+    }
+  } else {  
+    // Step. a <= b
+    //   IH: sum(a+1, b, K => k) = (b*(b+1) + (a+1)*(1-(a+1)))/2 
+    //    T: sum(a, b, k => k)   = (b*(b+1) + a*(1-a))/2 
+    calc {  
+         sum(a, b, k => k);
+      == { reveal sum(); }
+         a + sum(a+1, b, k => k);
+      == { lem_sum_interval(a+1, b); }  // by IH
+         a + (b*(b+1) + (a+1)*(1-(a+1)))/2;
+      == (b*(b+1) + a*(1-a))/2;            
+    }
+  }
+}
+
+// Following sum lemmas are only stated for integer sum
+
+// sum_{k=1}^{n}k = (n*(n+1))/2 
+lemma lem_sum_triangle(n:nat)
+  ensures sum(1, n, k => k) == (n*(n+1))/2
+{
+  lem_sum_interval(1, n);
+}
+
+// a <= b+1 ==> sum_{k=a}^{b}(b-k+a) = sum_{k=a}^{b}k
+lemma {:axiom} lem_sum_revIndex(a:int, b:int)
+  requires a <= b+1
+  ensures  sum(a, b, k => b-k+a) == sum(a, b, k => k)
+
+
+/**************************************************************************
+  Sum over sequences
+**************************************************************************/
+
+opaque ghost function sumSeq(s:seq<int>, f:int->real): real
+  decreases s
+{
+  if |s| == 0 
+  then 0.0
+  else f(s[0]) + sumSeq(s[1..], f)
+}
+
+/**************************************************************************
+  Sum over sets
+**************************************************************************/
+
+opaque ghost function sumSet(s:set<int>, f:int->real): real
+  decreases s
+{
+  if |s| == 0 
+  then 0.0
+  else var x :| x in s;
+       f(x) + sumSet(s - {x}, f)
+}
